Do not use Scopes for Step

Strata/DL/Lambda/Semantics.lean
@@ -18,6 +18,16 @@ variable {IDMeta:Type} [DecidableEq IDMeta]
 open Lambda
 
 /--
+A free variable -> expressions mapping.
+-/
+abbrev FreeVarMap := Map (Identifier IDMeta) (LExpr LMonoTy IDMeta)
+
+@[reducible]
+def Scopes.toFreeVarMap (s:Scopes IDMeta)
+    : Map (Identifier IDMeta) (LExpr LMonoTy IDMeta) :=
+  (List.flatten s).map (fun (id,(_,e)) => (id,e))
+
+/--
 A small-step semantics of LExpr.
 Currently only defined for LMonoTy, but it will be expanded to an arbitrary
 type.
@@ -27,47 +37,47 @@ This small-step definitions faithfully follows the behavior of LExpr.eval,
 except that this inductive definition may stuck early when there is no
 assignment to a free variable available in LState.
 -/
-inductive Step (F:@Factory IDMeta) (state:Scopes IDMeta)
+inductive Step (F:@Factory IDMeta) (rf:FreeVarMap)
   : LExpr LMonoTy IDMeta → LExpr LMonoTy IDMeta → Prop where
 -- A free variable. Stuck if fvar does not exist in LState.
 | expand_fvar:
   ∀ (x:Identifier IDMeta) (e:LExpr LMonoTy IDMeta),
-    state.find? x = .some (ty,e) →
-    Step F state (.fvar x ty') e
+    rf.find? x = .some e →
+    Step F rf (.fvar x ty) e
 
 -- Beta reduction for lambda; Call-by-value semantics.
 | beta:
   ∀ (e1 v2:LExpr LMonoTy IDMeta),
     LExpr.isCanonicalValue F v2 →
-    Step F state (.app (.abs ty e1) v2) (LExpr.subst v2 e1)
+    Step F rf (.app (.abs ty e1) v2) (LExpr.subst v2 e1)
 
 -- Call-by-value semantics.
 | reduce_2:
   ∀ (v1 e2 e2':LExpr LMonoTy IDMeta),
     LExpr.isCanonicalValue F v1 →
-    Step F state e2 e2' →
-    Step F state (.app v1 e2) (.app v1 e2')
+    Step F rf e2 e2' →
+    Step F rf (.app v1 e2) (.app v1 e2')
 
 | reduce_1:
   ∀ (e1 e1' e2:LExpr LMonoTy IDMeta),
-    Step F state  e1 e1' →
-    Step F state  (.app e1 e2) (.app e1' e2)
+    Step F rf e1 e1' →
+    Step F rf (.app e1 e2) (.app e1' e2)
 
 -- For ite x e1 e2, do not eagerly evaluate e1 and e2.
 -- For the reduction order, ite x e1 e2 is interpreted as
 -- 'ite x (λ.e1) (λ.e2)'.
 | ite_reduce_then:
   ∀ (ethen eelse:LExpr LMonoTy IDMeta),
-    Step F state  (.ite (.const (.boolConst true)) ethen eelse) ethen
+    Step F rf (.ite (.const (.boolConst true)) ethen eelse) ethen
 
 | ite_reduce_else:
   ∀ (ethen eelse:LExpr LMonoTy IDMeta),
-    Step F state  (.ite (.const (.boolConst false)) ethen eelse) eelse
+    Step F rf (.ite (.const (.boolConst false)) ethen eelse) eelse
 
 | ite_reduce_cond:
   ∀ (econd econd' ethen eelse:LExpr LMonoTy IDMeta),
-    Step F state  econd econd' →
-    Step F state  (.ite econd ethen eelse) (.ite econd' ethen eelse)
+    Step F rf econd econd' →
+    Step F rf (.ite econd ethen eelse) (.ite econd' ethen eelse)
 
 -- Equality. Reduce after both operands evaluate to values.
 | eq_reduce:
@@ -75,24 +85,24 @@ inductive Step (F:@Factory IDMeta) (state:Scopes IDMeta)
     (H1:LExpr.isCanonicalValue F e1)
     (H2:LExpr.isCanonicalValue F e2),
     eres = .const (.boolConst (LExpr.eql F e1 e2 H1 H2)) →
-    Step F state  (.eq e1 e2) eres
+    Step F rf (.eq e1 e2) eres
 
 | eq_reduce_lhs:
   ∀ (e1 e1' e2:LExpr LMonoTy IDMeta),
-    Step F state  e1 e1' →
-    Step F state  (.eq e1 e2) (.eq e1' e2)
+    Step F rf e1 e1' →
+    Step F rf (.eq e1 e2) (.eq e1' e2)
 
 | eq_reduce_rhs:
   ∀ (v1 e2 e2':LExpr LMonoTy IDMeta),
     LExpr.isCanonicalValue F v1 →
-    Step F state  e2 e2' →
-    Step F state  (.eq v1 e2) (.eq v1 e2')
+    Step F rf e2 e2' →
+    Step F rf (.eq v1 e2) (.eq v1 e2')
 
 -- Evaluation keeps the metadata.
 | mdata:
   ∀ (e e':LExpr LMonoTy IDMeta) (m:Info),
-    Step F state  e e' →
-    Step F state  (.mdata m e) (.mdata m e')
+    Step F rf e e' →
+    Step F rf (.mdata m e) (.mdata m e')
 
 -- Expand functions and free variables when they are evaluated.
 -- If the function body is unknown, concreteEval can be instead used. Look at
@@ -104,7 +114,7 @@ inductive Step (F:@Factory IDMeta) (state:Scopes IDMeta)
     args.all (LExpr.isCanonicalValue F) →
     fn.body = .some fnbody →
     new_body = LExpr.substFvars fnbody (fn.inputs.keys.zip args) →
-    Step F state  e new_body
+    Step F rf e new_body
 
 -- The second way of evaluating a function call.
 -- If LFunc has a concrete evaluator, this can be used to 'jump' to the final
@@ -114,12 +124,12 @@ inductive Step (F:@Factory IDMeta) (state:Scopes IDMeta)
     F.callOfLFunc e = .some (callee,args,fn) →
     args.all (LExpr.isCanonicalValue F) →
     fn.concreteEval = .some denotefn →
-    Step F state  e (denotefn (LExpr.mkApp callee args) args)
+    Step F rf e (denotefn (LExpr.mkApp callee args) args)
 
 
 theorem step_const_stuck:
-  ∀ (F:@Factory IDMeta) (state:Scopes IDMeta) x e,
-  ¬ Step F state  (.const x) e := by
+  ∀ (F:@Factory IDMeta) r x e,
+  ¬ Step F r (.const x) e := by
   intros
   intro H
   contradiction
@@ -127,10 +137,10 @@ theorem step_const_stuck:
 /--
 Multi-step execution: reflexive transitive closure of single steps.
 -/
-inductive StepStar (F:@Factory IDMeta) (state:Scopes IDMeta)
+inductive StepStar (F:@Factory IDMeta) (rf:@FreeVarMap IDMeta)
   : LExpr LMonoTy IDMeta → LExpr LMonoTy IDMeta → Prop where
-| refl : StepStar F state e e
-| step : ∀ e e' e'', Step F state e e' → StepStar F state e' e''
-        → StepStar F state e e''
+| refl : StepStar F rf e e
+| step : ∀ e e' e'', Step F rf e e' → StepStar F rf e' e''
+        → StepStar F rf e e''
 
 end Lambda
